Typing relation(s)

theories/abs_imp.v
@@ -8,19 +8,21 @@ From stdpp Require Export
   relations
 .
 From ABS Require Import abs_defs
-  utils.
+utils
+abs_functional_metatheory
+.
 
 Tactic Notation "simp" := simplify_map_eq.
 Tactic Notation "is_eq" ident(a) ident(b) :=
   destruct (decide (a = b)) as [<- | ?].
 
-Definition f : Set := nat. (*r future identifier *)
+Definition f : Set := string. (*r future names *)
 Lemma eq_f: forall (x y : f), {x = y} + {x <> y}.
 Proof.
   decide equality; auto with ott_coq_equality arith.
 Defined.
 
-Definition o : Set := nat. (*r object identifier *)
+Definition o : Set := string. (*r object names *)
 Lemma eq_o: forall (x y : o), {x = y} + {x <> y}.
 Proof.
   decide equality; auto with ott_coq_equality arith.
@@ -28,6 +30,12 @@ Defined.
 
 Definition m : Set := string. (*r method names *)
 Lemma eq_m: forall (x y : m), {x = y} + {x <> y}.
+Proof.
+  decide equality; auto with ott_coq_equality arith.
+Defined.
+
+Definition C : Set := string. (*r class names *)
+Lemma eq_C: forall (x y : C), {x = y} + {x <> y}.
 Proof.
   decide equality; auto with ott_coq_equality arith.
 Defined.
@@ -46,6 +54,19 @@ Inductive stmt : Set :=
 | stmt_cond (e0:e) (s1 s2: stmt)
 | stmt_loop (e0:e) (s: stmt)
 | stmt_ret (e0:e).
+
+Variant M : Set :=  (*r method definition *)
+ | M_m (T_5:T) (m0:m) (params decl:list (T*x)) (body:stmt).
+
+(* Class definition *)
+Variant CL: Set :=
+  | class (name:C) (_: list(T*x)) (_: list M).
+
+Equations get_class_name (CL0:CL): C := {get_class_name (class name _ _) := name}.
+Equations get_fields (CL0:CL): list (T*x) := {get_fields (class _ fields _) := fields}.
+
+Variant P: Set :=
+  | program (_: list CL) (decl : list (T*x)) (main: stmt).
 
 Lemma cons_neq{X:Type}: forall (x:X) l, x :: l <> l.
 Proof.
@@ -96,7 +117,7 @@ Proof.
   apply prod_eq_dec.
 Qed.
 
-Inductive task: Set := tsk (p:stmt) (l:s) (destiny:f).
+Variant task: Set := tsk (p:stmt) (l:s).
 
 #[global]
 Instance s_eq_dec: EqDecision s.
@@ -117,13 +138,35 @@ Admitted.
 Notation queue := (gmultiset task).
 
 Inductive cn: Set :=
-| cn_future (*f0:f*) (v:option t)
-| cn_object (*o0:o*) (a:s) (p:option task) (q: queue)
+| cn_future (f0:f) (v:option t)
+| cn_object (C0:C) (a:s) (p:option task) (q: queue)
 | cn_invoc (o0:o) (f0:f) (m0:m) (vs: list t).
 
 Notation config := (natmap cn).
 Definition add (p:task) (q:queue) := q ⊎ {[+ p +]}.
 Definition remove (p:task) (q:queue) := difference q {[+ p +]}.
+
+Equations get_method_decl (m0:m) (l: list M) : option M := {
+  get_method_decl _ [] := None ;
+  get_method_decl m ((M_m T m' params decl body)::Ms) :=
+      if String.eqb m m' then Some (M_m T m' params decl body) else get_method_decl m Ms
+  }.
+
+Equations bind_params_aux (s0:s) (vs: list t) (params: list (T*x)): s := {
+  bind_params_aux s0 [] _ := s0;
+  bind_params_aux s0 _ [] := s0;
+  bind_params_aux s0 (v::vs) ((_,x)::Txs) := insert x v (bind_params_aux s0 vs Txs)
+  }.
+Definition bind_params := bind_params_aux empty.
+
+Equations bind (m0:m) (vs: list t) (f0:f) (CL0:CL) : option task := {
+  bind m vs f (class n params m_list) :=
+  match get_method_decl m m_list with
+  | None => None
+  | Some (M_m T m' params decl body) =>
+      Some (tsk body (bind_params vs params))
+  end
+  }.
 
 Definition reduce (Fs: list F): relation (e * s) :=
   fun  x y => let (e0, s0) := x in let (e1, s1) := y in red_e Fs s0 e0 s1 e1.
@@ -141,68 +184,178 @@ Instance elem_of_map: ElemOf x s := fun x s => s !! x <> None.
 #[global]
 Instance elem_of_config: ElemOf nat config := fun x s => s !! x <> None.
 
-Inductive stmt_step (Fs:list F) : config -> config -> Prop :=
-| step_activate: forall σ p q o a,
-    p ∈ q ->
-    σ !! o = Some (cn_object a None q) ->
-    stmt_step Fs σ (<[o:=(cn_object a (Some p) (remove p q))]> σ)
+Definition destiny: f := "destiny"%string.
 
-| step_asgn1: forall σ o a l destiny x e s q v,
+Inductive stmt_step (Fs:list F): list CL -> config -> config -> Prop :=
+| step_activate: forall Cs σ p q i a C,
+    p ∈ q ->
+    σ !! i = Some (cn_object C a None q) ->
+    stmt_step Fs Cs σ (<[i:=(cn_object C a (Some p) (remove p q))]> σ)
+
+| step_asgn1: forall Cs σ i a C l x e s q v,
     x ∈ l ->
     eval Fs (union a l) e v ->
-    σ !! o = Some (cn_object a (Some (tsk (stmt_seq (stmt_asgn x (rhs_e e)) s) l destiny)) q) ->
-    stmt_step Fs σ (<[o:=(cn_object a (Some (tsk s (<[x:=v]> l) destiny)) q)]> σ)
+    σ !! i = Some (cn_object C a (Some (tsk (stmt_seq (stmt_asgn x (rhs_e e)) s) l)) q) ->
+    stmt_step Fs Cs σ (<[i:=(cn_object C a (Some (tsk s (<[x:=v]> l))) q)]> σ)
 
-| step_asgn2: forall σ o a l destiny x e s q v,
+| step_asgn2: forall Cs σ o a C l x e s q v,
     ~ x ∈ l ->
     eval Fs (union a l) e v ->
-    σ !! o = Some (cn_object a (Some (tsk (stmt_seq (stmt_asgn x (rhs_e e)) s) l destiny)) q) ->
-    stmt_step Fs σ (<[o:=(cn_object (<[x:=v]> a) (Some (tsk s l destiny)) q)]> σ)
+    σ !! o = Some (cn_object C a (Some (tsk (stmt_seq (stmt_asgn x (rhs_e e)) s) l)) q) ->
+    stmt_step Fs Cs σ (<[o:=(cn_object C (<[x:=v]> a) (Some (tsk s l)) q)]> σ)
 
-| step_cond1: forall σ o a l destiny e s1 s2 s q,
+| step_cond1: forall Cs σ o a C l e s1 s2 s q,
     eval Fs (union a l) e (t_b true) ->
-    σ !! o = Some (cn_object a (Some (tsk (stmt_seq (stmt_cond e s1 s2) s) l destiny)) q) ->
-    stmt_step Fs σ (<[o:=cn_object a (Some (tsk (stmt_seq s1 s) l destiny)) q]> σ)
+    σ !! o = Some (cn_object C a (Some (tsk (stmt_seq (stmt_cond e s1 s2) s) l)) q) ->
+    stmt_step Fs Cs σ (<[o:=cn_object C a (Some (tsk (stmt_seq s1 s) l)) q]> σ)
 
-| step_cond2: forall σ o a l destiny e s1 s2 s q,
+| step_cond2: forall Cs σ o a C l e s1 s2 s q,
     eval Fs (union a l) e (t_b false) ->
-    σ !! o = Some (cn_object a (Some (tsk (stmt_seq (stmt_cond e s1 s2) s) l destiny)) q) ->
-    stmt_step Fs σ (<[o:=cn_object a (Some (tsk (stmt_seq s2 s) l destiny)) q]> σ)
+    σ !! o = Some (cn_object C a (Some (tsk (stmt_seq (stmt_cond e s1 s2) s) l)) q) ->
+    stmt_step Fs Cs σ (<[o:=cn_object C a (Some (tsk (stmt_seq s2 s) l)) q]> σ)
 
-| step_skip1: forall σ o a l destiny s q,
-    σ !! o = Some (cn_object a (Some (tsk (stmt_seq stmt_skip s) l destiny)) q) ->
-    stmt_step Fs σ (<[o:=cn_object a (Some (tsk s l destiny)) q]> σ)
+| step_skip1: forall Cs σ o a C l s q,
+    σ !! o = Some (cn_object C a (Some (tsk (stmt_seq stmt_skip s) l)) q) ->
+    stmt_step Fs Cs σ (<[o:=cn_object C a (Some (tsk s l)) q]> σ)
 
-| step_skip2: forall σ o a l destiny q,
-    σ !! o = Some (cn_object a (Some (tsk stmt_skip l destiny)) q) ->
-    stmt_step Fs σ (<[o:=cn_object a None q]> σ)
+| step_skip2: forall Cs σ o a C l q,
+    σ !! o = Some (cn_object C a (Some (tsk stmt_skip l)) q) ->
+    stmt_step Fs Cs σ (<[o:=cn_object C a None q]> σ)
 
-| step_while: forall σ o a l destiny e s1 s2 q,
-    σ !! o = Some (cn_object a (Some (tsk (stmt_seq (stmt_loop e s1) s2) l destiny)) q) ->
-    stmt_step Fs σ (<[o:=cn_object a (Some ( tsk (stmt_seq (stmt_cond e (stmt_seq s1 (stmt_loop e s1)) stmt_skip) s2) l destiny)) q]> σ)
+| step_while: forall Cs σ o a C l e s1 s2 q,
+    σ !! o = Some (cn_object C a (Some (tsk (stmt_seq (stmt_loop e s1) s2) l)) q) ->
+    stmt_step Fs Cs σ (<[o:=cn_object C a (Some ( tsk (stmt_seq (stmt_cond e (stmt_seq s1 (stmt_loop e s1)) stmt_skip) s2) l)) q]> σ)
 
-| step_call: forall σ o o' a l destiny q x m es vs s f i,
-    ~ f ∈ σ ->
+| step_call: forall Cs σ oi o' a C l q x m es vs s f fi i,
+    ~ fi ∈ σ ->
     ~ i ∈ σ ->
     eval_list Fs (union a l) es vs ->
-    σ !! o = Some (cn_object a (Some (tsk (stmt_seq (stmt_asgn x (rhs_invoc o' m es)) s) l destiny)) q) ->
-    stmt_step Fs σ (<[o:=cn_object a (Some (tsk (stmt_seq (stmt_asgn x (rhs_get f)) s) l destiny)) q]>
+    σ !! oi = Some (cn_object C a (Some (tsk (stmt_seq (stmt_asgn x (rhs_invoc o' m es)) s) l)) q) ->
+    stmt_step Fs Cs σ (<[oi:=cn_object C a (Some (tsk (stmt_seq (stmt_asgn x (rhs_get f)) s) l)) q]>
                       (<[i:=cn_invoc o' f m vs]>
-                         (<[f:=cn_future None]> σ)))
+                         (<[fi:=cn_future f None]> σ)))
 
-| step_return: forall σ o a l destiny e v q f,
+| step_return: forall Cs σ o a C l e v q f fi,
     eval Fs (union a l) e v ->
-    σ !! f = Some (cn_future None) ->
-    σ !! o = Some (cn_object a (Some (tsk (stmt_ret e) l destiny)) q) ->
-    stmt_step Fs σ (<[o:=cn_object a None q]>
-                      (<[f:=cn_future (Some v)]> σ))
-| step_read: forall σ o a l destiny x s v q f,
-    σ !! f = Some (cn_future (Some v)) ->
-    σ !! o = Some (cn_object a (Some (tsk (stmt_seq (stmt_asgn x (rhs_get f)) s) l destiny)) q) ->
-    stmt_step Fs σ (<[o:=cn_object a (Some (tsk (stmt_seq (stmt_asgn x (rhs_e (e_t v))) s) l destiny)) q]> σ)
-(*missing: load because it requires resolving method names to objects > something like typ_F?*)
+    σ !! fi = Some (cn_future f None) ->
+    σ !! o = Some (cn_object C a (Some (tsk (stmt_ret e) l)) q) ->
+    l !! destiny = Some (t_fut fi) ->
+    stmt_step Fs Cs σ (<[o:=cn_object C a None q]>
+                      (<[fi:=cn_future f (Some v)]> σ))
+
+| step_read: forall Cs σ o a C l x s v q f fi,
+    σ !! fi = Some (cn_future f (Some v)) ->
+    σ !! o = Some (cn_object C a (Some (tsk (stmt_seq (stmt_asgn x (rhs_get f)) s) l)) q) ->
+    stmt_step Fs Cs σ (<[o:=cn_object C a (Some (tsk (stmt_seq (stmt_asgn x (rhs_e (e_t v))) s) l)) q]> σ)
+
+| step_load: forall σ o oi i a p p' q f m vs C CL Cs Cs',
+    σ !! oi = Some (cn_object C a p q) ->
+    σ !! i = Some (cn_invoc o f m vs) ->
+    get_class_name CL = C ->
+    bind m vs f CL = Some p' ->
+    stmt_step Fs (Cs ++ [CL] ++ Cs') σ
+    (<[oi:=cn_object C a p (add p' q)]>
+       (delete i σ))
 .
 
-(*TODO: typing judgement for stmt *)
+(** Typing *)
+Inductive typ_method: list CL -> G -> C -> m -> list e -> T -> Prop :=
+(* TODO: implement this *).
+Inductive typ_CL: G -> CL -> Prop :=
+(* TODO: implement this *).
+
+Inductive typ_rhs (Cs: list CL): G -> rhs -> ctxv -> Prop :=
+| typ_rhs_e: forall G e T,
+    typ_e G e T ->
+    typ_rhs Cs G (rhs_e e) (ctxv_T T)
+| typ_rhs_invoc: forall G o m es T,
+    typ_method Cs G o m es T ->
+    typ_rhs Cs G (rhs_invoc o m es) (ctxv_fut T)
+| typ_rhs_get: forall G f T,
+    G !! f = Some (ctxv_fut T) ->
+    typ_rhs Cs G (rhs_get f) (ctxv_T T)
+.
+
+Inductive typ_stmt (Cs: list CL): G -> stmt -> Prop :=
+| typ_stmt_seq: forall G s1 s2,
+    typ_stmt Cs G s1 ->
+    typ_stmt Cs G s2 ->
+    typ_stmt Cs G (stmt_seq s1 s2)
+
+| typ_stmt_skip: forall G,
+    typ_stmt Cs G stmt_skip
+
+|typ_stmt_asgn: forall G x r T,
+    G !! x = Some T ->
+    typ_rhs Cs G r T ->
+    typ_stmt Cs G (stmt_asgn x r)
+
+| typ_stmt_cond: forall G b s1 s2,
+    typ_e G b T_bool ->
+    typ_stmt Cs G s1 ->
+    typ_stmt Cs G s2 ->
+    typ_stmt Cs G (stmt_cond b s1 s2)
+
+| typ_stmt_loop: forall G b s,
+    typ_e G b T_bool ->
+    typ_stmt Cs G s ->
+    typ_stmt Cs G (stmt_loop b s)
+
+| typ_stmt_return: forall G e T,
+    typ_e G e T ->
+    G !! destiny = Some (ctxv_fut T) ->
+    typ_stmt Cs G (stmt_ret e)
+.
+
+Definition class_of: o -> C.
+Admitted.
+
+Equations task_well_typed (Cs: list CL) (G0:G) (t:task): Prop := {
+  task_well_typed Cs G0 (tsk p l) := G_vdash_s G0 l /\ typ_stmt Cs G0 p
+  }.
+(* this is a bit weird: the paper treats l sometimes as a list of typed variable bindings and sometimes as local state :/
+ if variable bindings then the typ_stmt judgement here should bind those vars in G0 *)
+
+Definition queue_well_typed (Cs: list CL) (G0:G) (q:queue): Prop :=
+  forall t, t ∈ q -> task_well_typed Cs G0 t.
+
+Inductive cn_well_typed (Cs: list CL): G -> cn -> Prop :=
+| wt_future_none: forall G f T,
+    G !! f = Some (ctxv_fut T) ->
+    cn_well_typed Cs G (cn_future f None)
+
+| wt_future_some: forall G f t T,
+    G !! f = Some (ctxv_fut T) ->
+    typ_e G (e_t t) T ->
+    cn_well_typed Cs G (cn_future f (Some t))
+
+| wt_invoc: forall G o f m vs T,
+    typ_method Cs G (class_of o) m (map e_t vs) T ->
+    G !! f = Some (ctxv_fut T) ->
+    cn_well_typed Cs G (cn_invoc o f m vs)
+
+| wt_object_none: forall G C a q,
+    queue_well_typed Cs G q ->
+    cn_well_typed Cs G (cn_object C a None q)
+
+| wt_object_some: forall G C a p q,
+    queue_well_typed Cs G q ->
+    task_well_typed Cs G p ->
+    cn_well_typed Cs G (cn_object C a (Some p) q)
+.
+
+Definition config_well_typed (Cs: list CL) (G0:G) (conf: config) :=
+  forall i ob, conf !! i = Some ob -> cn_well_typed Cs G0 ob.
+
+Theorem type_preservation : forall (Fs: list F) (Cs: list CL) (G0: G),
+  Forall (typ_F G0) Fs ->
+  Forall (typ_CL G0) Cs ->
+  forall σ σ',
+    config_well_typed Cs G0 σ ->
+    stmt_step Fs Cs σ σ' ->
+    exists G',
+      G0 ⊆ G' /\ config_well_typed Cs G' σ'.
+Admitted.
+
 (*TODO: subject reduction for stmt_step *)
 (*TODO: labels + traces? *)
